Simplify init printing

examples/boardroomVoting/BoardroomVotingExtractionCameLIGO.v
@@ -48,6 +48,27 @@ Definition setupWchain := (BV.Setup × Chain).
 
 Definition init_wrapper (cctx : ContractCallContext) (s : setupWchain) := (run_contract_initer BV.init) s.2 cctx s.1.
 
+
+(** In the Tezos blockchain there is no concept of initialisation
+    function. However, it's common to provide a function that computes
+    a valid initial storage that can be used for deployment.*)
+Definition init (s : Address * Setup) : option State :=
+  if (finish_registration_by s.2 <? finish_vote_by s.2)%nat
+      then
+        Some {| owner := s.1;
+                registered_voters := AddressMap.empty;
+                public_keys := [];
+                setup := s.2;
+               tally := None; |}
+      else None.
+
+Lemma init_eq_init_wrapper cctx s :
+  init_wrapper cctx s = init (cctx.(ctx_from), s.1).
+Proof.
+  unfold init_wrapper,init. cbn.
+  now destruct (_ <? _)%nat.
+Qed.
+
 Definition receive_wrapper (c : Chain)
                            (ctx : ContractCallContext)
                            (st : BV.State) 
@@ -117,7 +138,7 @@ Definition hash_func_def := "let hash_func (l :  (nat) list) = addN 1n (List.fol
 Definition callctx := "(Tezos.sender,(Tezos.self_address,(Tezos.amount,Tezos.balance)))".
 
 
-Definition BV_MODULE : CameLIGOMod BV.Msg ContractCallContext setupWchain BV.State ActionBody :=
+Definition BV_MODULE : CameLIGOMod BV.Msg ContractCallContext (Address * Setup) BV.State ActionBody :=
   {| (* a name for the definition with the extracted code *)
     lmd_module_name := "cameligo_boardroomvoting" ;
 
@@ -125,7 +146,7 @@ Definition BV_MODULE : CameLIGOMod BV.Msg ContractCallContext setupWchain BV.Sta
     lmd_prelude := concat nl [CameLIGOPretty.CameLIGOPrelude; extra_ops; hash_func_def];
 
     (* initial storage *)
-    lmd_init := init_wrapper;
+    lmd_init := init;
 
     (* no extra operations in [init] are required *)
     lmd_init_prelude := "";
